don't use List.length

src/Init/Data/Iterators/Combinators/Monadic/Take.lean
@@ -25,11 +25,16 @@ variable {α : Type w} {m : Type w → Type w'} {β : Type w}
 The internal state of the `IterM.take` iterator combinator.
 -/
 @[unbox]
-structure Take (α : Type w) (m : Type w → Type w') (β : Type w) where
-  /-- Internal implementation detail of the iterator library -/
-  remaining : Nat
+structure Take (α : Type w) (m : Type w → Type w') {β : Type w} [Iterator α m β] where
+  /--
+  Internal implementation detail of the iterator library.
+  Caution: For `take n`, `countdown` is `n + 1`.
+  If `countdown` is zero, the combinator only terminates when `inner` terminates.
+  -/
+  countdown : Nat
   /-- Internal implementation detail of the iterator library -/
   inner : IterM (α := α) m β
+  finite : countdown > 0 ∨ Finite α m
 
 /--
 Given an iterator `it` and a natural number `n`, `it.take n` is an iterator that outputs
@@ -55,97 +60,160 @@ it.take 3   ---a--⊥
 This combinator incurs an additional O(1) cost with each output of `it`.
 -/
 @[always_inline, inline]
-def IterM.take (n : Nat) (it : IterM (α := α) m β) :=
-  toIterM (Take.mk n it) m β
+def IterM.take [Iterator α m β] (n : Nat) (it : IterM (α := α) m β) :=
+  toIterM (Take.mk (n + 1) it (Or.inl <| Nat.zero_lt_succ _)) m β
 
-theorem IterM.take.surjective {α : Type w} {m : Type w → Type w'} {β : Type w}
-    (it : IterM (α := Take α m β) m β) :
+/--
+This combinator is only useful for advanced use cases.
+
+Given a finite iterator `it`, returns an iterator that behaves exactly like `it` but is of the same
+type as `it.take n`.
+
+**Marble diagram:**
+
+```text
+it          ---a----b---c--d-e--⊥
+it.toTake   ---a----b---c--d-e--⊥
+```
+
+**Termination properties:**
+
+* `Finite` instance: always
+* `Productive` instance: always
+
+**Performance:**
+
+This combinator incurs an additional O(1) cost with each output of `it`.
+-/
+@[always_inline, inline]
+def IterM.toTake [Iterator α m β] [Finite α m] (it : IterM (α := α) m β) :=
+  toIterM (Take.mk 0 it (Or.inr inferInstance)) m β
+
+theorem IterM.take.surjective_of_zero_lt {α : Type w} {m : Type w → Type w'} {β : Type w}
+    [Iterator α m β] (it : IterM (α := Take α m) m β) (h : 0 < it.internalState.countdown) :
     ∃ (it₀ : IterM (α := α) m β) (k : Nat), it = it₀.take k := by
-  refine ⟨it.internalState.inner, it.internalState.remaining, rfl⟩
+  refine ⟨it.internalState.inner, it.internalState.countdown - 1, ?_⟩
+  simp only [take, Nat.sub_add_cancel (m := 1) (n := it.internalState.countdown) (by omega)]
+  rfl
 
-inductive Take.PlausibleStep [Iterator α m β] (it : IterM (α := Take α m β) m β) :
-    (step : IterStep (IterM (α := Take α m β) m β) β) → Prop where
-  | yield : ∀ {it' out k}, it.internalState.inner.IsPlausibleStep (.yield it' out) →
-      it.internalState.remaining = k + 1 → PlausibleStep it (.yield (it'.take k) out)
-  | skip : ∀ {it' k}, it.internalState.inner.IsPlausibleStep (.skip it') →
-      it.internalState.remaining = k + 1 → PlausibleStep it (.skip (it'.take (k + 1)))
+inductive Take.PlausibleStep [Iterator α m β] (it : IterM (α := Take α m) m β) :
+    (step : IterStep (IterM (α := Take α m) m β) β) → Prop where
+  | yield : ∀ {it' out}, it.internalState.inner.IsPlausibleStep (.yield it' out) →
+      (h : it.internalState.countdown ≠ 1) → PlausibleStep it (.yield ⟨it.internalState.countdown - 1, it', it.internalState.finite.imp_left (by omega)⟩ out)
+  | skip : ∀ {it'}, it.internalState.inner.IsPlausibleStep (.skip it') →
+      it.internalState.countdown ≠ 1 → PlausibleStep it (.skip ⟨it.internalState.countdown, it', it.internalState.finite⟩)
   | done : it.internalState.inner.IsPlausibleStep .done → PlausibleStep it .done
-  | depleted : it.internalState.remaining = 0 →
+  | depleted : it.internalState.countdown = 1 →
       PlausibleStep it .done
 
 @[always_inline, inline]
-instance Take.instIterator [Monad m] [Iterator α m β] : Iterator (Take α m β) m β where
+instance Take.instIterator [Monad m] [Iterator α m β] : Iterator (Take α m) m β where
   IsPlausibleStep := Take.PlausibleStep
   step it :=
-    match h : it.internalState.remaining with
-    | 0 => pure <| .deflate <| .done (.depleted h)
-    | k + 1 => do
+    if h : it.internalState.countdown = 1 then
+      pure <| .deflate <| .done (.depleted h)
+    else do
       match (← it.internalState.inner.step).inflate with
-      | .yield it' out h' => pure <| .deflate <| .yield (it'.take k) out (.yield h' h)
-      | .skip it' h' => pure <| .deflate <| .skip (it'.take (k + 1)) (.skip h' h)
+      | .yield it' out h' =>
+        pure <| .deflate <| .yield ⟨it.internalState.countdown - 1, it', (it.internalState.finite.imp_left (by omega))⟩ out (.yield h' h)
+      | .skip it' h' => pure <| .deflate <| .skip ⟨it.internalState.countdown, it', it.internalState.finite⟩ (.skip h' h)
       | .done h' => pure <| .deflate <| .done (.done h')
 
 def Take.Rel (m : Type w → Type w') [Monad m] [Iterator α m β] [Productive α m] :
-    IterM (α := Take α m β) m β → IterM (α := Take α m β) m β → Prop :=
-  InvImage (Prod.Lex Nat.lt_wfRel.rel IterM.TerminationMeasures.Productive.Rel)
-    (fun it => (it.internalState.remaining, it.internalState.inner.finitelyManySkips))
+    IterM (α := Take α m) m β → IterM (α := Take α m) m β → Prop :=
+  open scoped Classical in
+  if _ : Finite α m then
+    InvImage (Prod.Lex Nat.lt_wfRel.rel IterM.TerminationMeasures.Finite.Rel)
+      (fun it => (it.internalState.countdown, it.internalState.inner.finitelyManySteps))
+  else
+    InvImage (Prod.Lex Nat.lt_wfRel.rel IterM.TerminationMeasures.Productive.Rel)
+      (fun it => (it.internalState.countdown, it.internalState.inner.finitelyManySkips))
 
-theorem Take.rel_of_remaining [Monad m] [Iterator α m β] [Productive α m]
-    {it it' : IterM (α := Take α m β) m β}
-    (h : it'.internalState.remaining < it.internalState.remaining) : Take.Rel m it' it :=
-  Prod.Lex.left _ _ h
+theorem Take.rel_of_countdown [Monad m] [Iterator α m β] [Productive α m]
+    {it it' : IterM (α := Take α m) m β}
+    (h : it'.internalState.countdown < it.internalState.countdown) : Take.Rel m it' it := by
+  simp only [Rel]
+  split <;> exact Prod.Lex.left _ _ h
 
 theorem Take.rel_of_inner [Monad m] [Iterator α m β] [Productive α m] {remaining : Nat}
     {it it' : IterM (α := α) m β}
     (h : it'.finitelyManySkips.Rel it.finitelyManySkips) :
-    Take.Rel m (it'.take remaining) (it.take remaining) :=
-  Prod.Lex.right _ h
+    Take.Rel m (it'.take remaining) (it.take remaining) := by
+  simp only [Rel]
+  split
+  · exact Prod.Lex.right _ (.of_productive h)
+  · exact Prod.Lex.right _ h
+
+theorem Take.rel_of_zero_of_inner [Monad m] [Iterator α m β]
+    {it it' : IterM (α := Take α m) m β}
+    (h : it.internalState.countdown = 0) (h' : it'.internalState.countdown = 0)
+    (h'' : haveI := it.internalState.finite.resolve_left (by omega); it'.internalState.inner.finitelyManySteps.Rel it.internalState.inner.finitelyManySteps) :
+    haveI := it.internalState.finite.resolve_left (by omega)
+    Take.Rel m it' it := by
+  haveI := it.internalState.finite.resolve_left (by omega)
+  simp only [Rel, this, ↓reduceDIte, InvImage, h, h']
+  exact Prod.Lex.right _ h''
 
 private def Take.instFinitenessRelation [Monad m] [Iterator α m β]
     [Productive α m] :
-    FinitenessRelation (Take α m β) m where
+    FinitenessRelation (Take α m) m where
   rel := Take.Rel m
   wf := by
-    apply InvImage.wf
-    refine ⟨fun (a, b) => Prod.lexAccessible (WellFounded.apply ?_ a) (WellFounded.apply ?_) b⟩
-    · exact WellFoundedRelation.wf
-    · exact WellFoundedRelation.wf
+    rw [Rel]
+    split
+    all_goals
+      apply InvImage.wf
+      refine ⟨fun (a, b) => Prod.lexAccessible (WellFounded.apply ?_ a) (WellFounded.apply ?_) b⟩
+      · exact WellFoundedRelation.wf
+      · exact WellFoundedRelation.wf
   subrelation {it it'} h := by
     obtain ⟨step, h, h'⟩ := h
     cases h'
     case yield it' out k h' h'' =>
       cases h
-      apply rel_of_remaining
-      simp_all [IterM.take]
+      cases it.internalState.finite
+      · apply rel_of_countdown
+        simp only
+        omega
+      · by_cases h : it.internalState.countdown = 0
+        · simp only [h, Nat.zero_le, Nat.sub_eq_zero_of_le]
+          apply rel_of_zero_of_inner h rfl
+          exact .single ⟨_, rfl, h'⟩
+        · apply rel_of_countdown
+          simp only
+          omega
     case skip it' out k h' h'' =>
       cases h
-      obtain ⟨it, k, rfl⟩ := IterM.take.surjective it
-      cases h''
-      apply Take.rel_of_inner
-      exact IterM.TerminationMeasures.Productive.rel_of_skip h'
+      by_cases h : it.internalState.countdown = 0
+      · simp only [h]
+        apply Take.rel_of_zero_of_inner h rfl
+        exact .single ⟨_, rfl, h'⟩
+      · obtain ⟨it, k, rfl⟩ := IterM.take.surjective_of_zero_lt it (by omega)
+        apply Take.rel_of_inner
+        exact IterM.TerminationMeasures.Productive.rel_of_skip h'
     case done _ =>
       cases h
     case depleted _ =>
       cases h
 
 instance Take.instFinite [Monad m] [Iterator α m β] [Productive α m] :
-    Finite (Take α m β) m :=
+    Finite (Take α m) m :=
   by exact Finite.of_finitenessRelation instFinitenessRelation
 
 instance Take.instIteratorCollect {n : Type w → Type w'} [Monad m] [Monad n] [Iterator α m β] :
-    IteratorCollect (Take α m β) m n :=
+    IteratorCollect (Take α m) m n :=
   .defaultImplementation
 
 instance Take.instIteratorCollectPartial {n : Type w → Type w'} [Monad m] [Monad n] [Iterator α m β] :
-    IteratorCollectPartial (Take α m β) m n :=
+    IteratorCollectPartial (Take α m) m n :=
   .defaultImplementation
 
 instance Take.instIteratorLoop {n : Type x → Type x'} [Monad m] [Monad n] [Iterator α m β] :
-    IteratorLoop (Take α m β) m n :=
+    IteratorLoop (Take α m) m n :=
   .defaultImplementation
 
 instance Take.instIteratorLoopPartial [Monad m] [Monad n] [Iterator α m β] :
-    IteratorLoopPartial (Take α m β) m n :=
+    IteratorLoopPartial (Take α m) m n :=
   .defaultImplementation
 
 end Std.Iterators
