src/Init/Data/Iterators/Combinators/Take.lean
@@ -36,8 +36,35 @@ it.take 3   ---a--⊥
 This combinator incurs an additional O(1) cost with each output of `it`.
 -/
 @[always_inline, inline]
-def Iter.take {α : Type w} {β : Type w} (n : Nat) (it : Iter (α := α) β) :
-    Iter (α := Take α Id β) β :=
+def Iter.take {α : Type w} {β : Type w} [Iterator α Id β] (n : Nat) (it : Iter (α := α) β) :
+    Iter (α := Take α Id) β :=
   it.toIterM.take n |>.toIter
+
+/--
+This combinator is only useful for advanced use cases.
+
+Given a finite iterator `it`, returns an iterator that behaves exactly like `it` but is of the same
+type as `it.take n`.
+
+**Marble diagram:**
+
+```text
+it          ---a----b---c--d-e--⊥
+it.toTake   ---a----b---c--d-e--⊥
+```
+
+**Termination properties:**
+
+* `Finite` instance: always
+* `Productive` instance: always
+
+**Performance:**
+
+This combinator incurs an additional O(1) cost with each output of `it`.
+-/
+@[always_inline, inline]
+def Iter.toTake {α : Type w} {β : Type w} [Iterator α Id β] [Finite α Id] (it : Iter (α := α) β) :
+    Iter (α := Take α Id) β :=
+  it.toIterM.toTake.toIter
 
 end Std.Iterators
