src/Init/Data/Iterators/Lemmas/Combinators/Monadic/Take.lean
@@ -13,16 +13,26 @@ public import Init.Data.Iterators.Lemmas.Consumers.Monadic
 
 namespace Std.Iterators
 
+theorem Take.isPlausibleStep_take_yield [Monad m] [Iterator α m β] {n : Nat}
+    {it : IterM (α := α) m β} (h : it.IsPlausibleStep (.yield it' out)) :
+    (it.take (n + 1)).IsPlausibleStep (.yield (it'.take n) out) :=
+  (.yield h (by simp [IterM.take]))
+
+theorem Take.isPlausibleStep_take_skip [Monad m] [Iterator α m β] {n : Nat}
+    {it : IterM (α := α) m β} (h : it.IsPlausibleStep (.skip it')) :
+    (it.take (n + 1)).IsPlausibleStep (.skip (it'.take (n + 1))) :=
+  (.skip h (by simp [IterM.take]))
+
 theorem IterM.step_take {α m β} [Monad m] [Iterator α m β] {n : Nat}
     {it : IterM (α := α) m β} :
     (it.take n).step = (match n with
       | 0 => pure <| .deflate <| .done (.depleted rfl)
       | k + 1 => do
         match (← it.step).inflate with
-        | .yield it' out h => pure <| .deflate <| .yield (it'.take k) out (.yield h rfl)
-        | .skip it' h => pure <| .deflate <| .skip (it'.take (k + 1)) (.skip h rfl)
+        | .yield it' out h => pure <| .deflate <| .yield (it'.take k) out (Take.isPlausibleStep_take_yield h)
+        | .skip it' h => pure <| .deflate <| .skip (it'.take (k + 1)) (Take.isPlausibleStep_take_skip h)
         | .done h => pure <| .deflate <| .done (.done h)) := by
-  simp only [take, step, Iterator.step, internalState_toIterM, Nat.succ_eq_add_one]
+  simp only [take, step, Iterator.step, internalState_toIterM]
   cases n
   case zero => rfl
   case succ k =>
@@ -31,11 +41,37 @@ theorem IterM.step_take {α m β} [Monad m] [Iterator α m β] {n : Nat}
     cases step.inflate using PlausibleIterStep.casesOn <;> rfl
 
 theorem IterM.toList_take_zero {α m β} [Monad m] [LawfulMonad m] [Iterator α m β]
-    [Finite (Take α m β) m]
-    [IteratorCollect (Take α m β) m m] [LawfulIteratorCollect (Take α m β) m m]
+    [Finite (Take α m) m]
+    [IteratorCollect (Take α m) m m] [LawfulIteratorCollect (Take α m) m m]
     {it : IterM (α := α) m β} :
     (it.take 0).toList = pure [] := by
   rw [toList_eq_match_step]
   simp [step_take]
+
+theorem IterM.step_toTake {α m β} [Monad m] [Iterator α m β] [Finite α m]
+    {it : IterM (α := α) m β} :
+    it.toTake.step = (do
+        match (← it.step).inflate with
+        | .yield it' out h => pure <| .deflate <| .yield it'.toTake out (.yield h Nat.zero_ne_one)
+        | .skip it' h => pure <| .deflate <| .skip it'.toTake (.skip h Nat.zero_ne_one)
+        | .done h => pure <| .deflate <| .done (.done h)) := by
+  simp only [toTake, step, Iterator.step, internalState_toIterM]
+  apply bind_congr
+  intro step
+  cases step.inflate using PlausibleIterStep.casesOn <;> rfl
+
+@[simp]
+theorem IterM.toList_toTake {α m β} [Monad m] [LawfulMonad m] [Iterator α m β] [Finite α m]
+    [IteratorCollect α m m] [LawfulIteratorCollect α m m]
+    {it : IterM (α := α) m β} :
+    it.toTake.toList = it.toList := by
+  induction it using IterM.inductSteps with | step it ihy ihs
+  rw [toList_eq_match_step, toList_eq_match_step]
+  simp only [step_toTake, bind_assoc]
+  apply bind_congr; intro step
+  cases step.inflate using PlausibleIterStep.casesOn
+  · simp [ihy ‹_›]
+  · simp [ihs ‹_›]
+  · simp
 
 end Std.Iterators
