src/Init/Data/Slice/List/Lemmas.lean
@@ -20,12 +20,17 @@ open Std.Iterators Std.PRange
 namespace Std.Slice.List
 
 theorem internalIter_rco_eq {α : Type u} {s : ListSlice α} :
-    Internal.iter s = s.internalRepresentation.list.iter.take s.internalRepresentation.stop := by
-  simp [Internal.iter, ToIterator.iter_eq]
+    Internal.iter s = match s.internalRepresentation.stop with
+        | some stop => s.internalRepresentation.list.iter.take stop
+        | none => s.internalRepresentation.list.iter.toTake := by
+  simp only [Internal.iter, ToIterator.iter_eq]; rfl
 
 theorem toList_internalIter {α : Type u} {s : ListSlice α} :
-    (Internal.iter s).toList = s.internalRepresentation.list.take s.internalRepresentation.stop := by
-  simp [internalIter_rco_eq]
+    (Internal.iter s).toList = match s.internalRepresentation.stop with
+        | some stop => s.internalRepresentation.list.take stop
+        | none => s.internalRepresentation.list := by
+  simp only [internalIter_rco_eq]
+  split <;> simp
 
 theorem internalIter_eq_toIteratorIter {α : Type u} {s : ListSlice α} :
     Internal.iter s = ToIterator.iter s :=
